Fix up the multi-argument introduction code
It now does functions and applications both.

Work on some of the compatibility lemmas for the logical relation (but
not the application one).

compiler/backend/clos_mtiScript.sml
@@ -3,11 +3,11 @@ open preamble closLangTheory;
 val _ = new_theory "clos_mti";
 
 val collect_args_def = Define `
-  (collect_args num_args (Fn loc fvs num_args' e) =
+  (collect_args num_args (Fn NONE NONE num_args' e) =
     if num_args + num_args' ≤ max_app then
       collect_args (num_args + num_args') e
     else
-      (max_app, Fn loc fvs (num_args + num_args' - max_app) e)) ∧
+      (max_app, Fn NONE NONE (num_args + num_args' - max_app) e)) ∧
   (collect_args num_args e = (num_args, e))`;
 
 val collect_args_ind = theorem"collect_args_ind";
@@ -61,11 +61,22 @@ val intro_multi_def = tDefine "intro_multi"`
     [Tick (HD (intro_multi [e]))]) ∧
   (intro_multi [Call n es] =
     [Call n (intro_multi es)]) ∧
-  (intro_multi [App loc e es] =
-    [App loc (HD (intro_multi [e])) (intro_multi es)]) ∧
-  (intro_multi [Fn loc fvs num_args e] =
+  (intro_multi [App NONE e1 es1] =
+    case HD (intro_multi [e1]) of
+    | App NONE e2 es2 =>
+      if LENGTH es1 + LENGTH es2 ≤ max_app then
+        [App NONE e2 (es2 ++ intro_multi es1)]
+      else
+        [App NONE (App NONE e2 (intro_multi es1)) es2]
+    | e1' => 
+        [App NONE e1' (intro_multi es1)]) ∧
+  (intro_multi [App (SOME l) e es] =
+    [App (SOME l) (HD (intro_multi [e])) (intro_multi es)]) ∧
+  (intro_multi [Fn NONE NONE num_args e] =
     let (num_args', e') = collect_args num_args e in
-      [Fn loc fvs num_args' (HD (intro_multi [e']))]) ∧
+      [Fn NONE NONE num_args' (HD (intro_multi [e']))]) ∧
+  (intro_multi [Fn loc fvs num_args e] =
+      [Fn loc fvs num_args (HD (intro_multi [e]))]) ∧
   (intro_multi [Letrec loc fvs funs e] =
     [Letrec loc fvs (MAP (\(num_args, e).
                            let (num_args', e') = collect_args num_args e in
@@ -92,14 +103,24 @@ val intro_multi_length = Q.store_thm("intro_multi_length",
   `!es. LENGTH (intro_multi es) = LENGTH es`,
   recInduct intro_multi_ind >>
   rw [intro_multi_def] >>
-  rw [intro_multi_def]);
-
-val intro_multi_sing = Q.prove (
-  `!e. ?e'. intro_multi [e] = [e']`,
-  Cases_on `e` >>
-  rw [intro_multi_def] >>
-  Cases_on `collect_args n e'` >>
+  Cases_on `intro_multi [e1]` >>
+  fs [] >>
+  every_case_tac >>
   fs []);
+
+val intro_multi_sing = Q.store_thm ("intro_multi_sing",
+  `!e. ?e'. intro_multi [e] = [e']`,
+  Induct_on `e` >>
+  rw [intro_multi_def] >>
+  TRY (qcase_tac `App loc e es` >> Cases_on `loc`) >>
+  TRY (qcase_tac `Fn loc vars num_args e` >> Cases_on `loc` >> Cases_on `vars`) >>
+  rw [intro_multi_def] >>
+  Cases_on `collect_args num_args e` >>
+  fs [] >>
+  Cases_on `e'` >>
+  simp [] >>
+  every_case_tac >>
+  rw []);
 
 val collect_args_idem = Q.prove (
   `!num_args e num_args' e'.
@@ -109,13 +130,27 @@ val collect_args_idem = Q.prove (
   ho_match_mp_tac collect_args_ind >>
   rw [collect_args_def, intro_multi_def] >>
   rw [collect_args_def, intro_multi_def] >>
-  fs [NOT_LESS_EQUAL] >>
-  `num_args'' = 0` by decide_tac >>
-  rw [] >>
-  imp_res_tac collect_args_zero >>
-  fs [] >>
-  `max_app< max_app` by decide_tac >>
-  fs []);
+  fs [NOT_LESS_EQUAL] 
+  >- (
+    rw [collect_args_def, intro_multi_def] >>
+    rw [collect_args_def, intro_multi_def] >>
+    TRY (`num_args'' = 0` by decide_tac) >>
+    rw [] >>
+    imp_res_tac collect_args_zero >>
+    fs [] >>
+    `max_app< max_app` by decide_tac >>
+    fs []) >>
+ qcase_tac `App loc e es` >>
+ Cases_on `loc` >>
+ rw [collect_args_def, intro_multi_def] >>
+ every_case_tac >>
+ rw [collect_args_def, intro_multi_def]);
+
+ (*
+val intro_multi_append = Q.store_thm ("intro_multi_append",
+`!es1 es2.
+  intro_multi (es1 ++ es2) = intro_multi es1 ++ intro_multi es2`,
+ cheat);
 
 val intro_multi_idem = Q.store_thm("intro_multi_idem",
   `!e. intro_multi (intro_multi e) = intro_multi e`,
@@ -132,7 +167,10 @@ val intro_multi_idem = Q.store_thm("intro_multi_idem",
   >- metis_tac [intro_multi_sing, HD]
   >- metis_tac [intro_multi_sing, HD]
   >- metis_tac [intro_multi_sing, HD]
+  >- cheat
   >- metis_tac [intro_multi_sing, HD]
+  >- metis_tac [intro_multi_sing, HD, collect_args_idem, PAIR_EQ]
+  >- metis_tac [intro_multi_sing, HD, collect_args_idem, PAIR_EQ]
   >- metis_tac [intro_multi_sing, HD, collect_args_idem, PAIR_EQ]
   >- (rw [LET_THM, MAP_MAP_o, combinTheory.o_DEF, UNCURRY] >>
       rw [MAP_EQ_f] >>
@@ -143,7 +181,8 @@ val intro_multi_idem = Q.store_thm("intro_multi_idem",
       res_tac >>
       rfs [] >>
       metis_tac [intro_multi_sing, HD, collect_args_idem, PAIR_EQ, FST, SND])
-  >- metis_tac [intro_multi_sing, HD]);
+  >- metis_tac [intro_multi_sing, HD, collect_args_idem]);
+  *)
 
 val _ = export_theory()
 
